WIP/ExtractSound.v
@@ -1,0 +1,409 @@
+From Stdlib Require Import Lists.List Classes.RelationClasses BinNums.
+Import ListNotations.
+From coqutil Require Import Map.Interface Map.Properties.
+From coqutil Require Import Datatypes.Result.
+From Utils Require Import Utils UnionFind Monad ExtraMaps VC Relations Result.
+From Utils.EGraph Require Import Defs Semantics.
+Import Monad.StateMonad.
+From Pyrosome.Theory Require Import Core ModelImpls.
+Import Core.Notations.
+From Pyrosome.Tools.EGraph Require Import Defs Theorems.
+
+Section Scratch.
+  Context (V : Type) {V_Eqb : Eqb V} {V_Eqb_ok : Eqb_ok V_Eqb}
+    {V_default : WithDefault V}.
+  Context (V_map : forall A, map.map V A)
+    (V_map_plus : ExtraMaps.map_plus V_map)
+    (V_map_ok : forall A, map.ok (V_map A))
+    (V_map_plus_ok : ExtraMaps.map_plus_ok V_map)
+    (V_trie : forall A, map.map (list V) A)
+    (V_trie_ok : forall A, map.ok (V_trie A)).
+  Context (succ : V -> V) (sort_of : V) (lt : V -> V -> Prop).
+  Context (lt_asymmetric : Asymmetric lt)
+    (lt_succ : forall x, lt x (succ x))
+    (lt_trans : Transitive lt).
+  Context (l : Rule.lang V) (wfl : wf_lang l) (sort_of_fresh : fresh sort_of l).
+
+  Local Notation lang_model := (lang_model V sort_of l).
+  Local Notation sound :=
+    (egraph_sound_for_interpretation V V V_map V_map V_trie (option positive) lang_model).
+  Local Notation egraph_ok := (egraph_ok V lt V V_map V_map V_trie (option positive)).
+
+  (* Clean reduction lemmas for the [stateT (V_map term) result] monad. *)
+  Lemma stateT_result_bind {A B} (f : A -> stateT (V_map (term V)) result B)
+    (m : stateT (V_map (term V)) result A) (s : V_map (term V)) :
+    Mbind f m s = match m s with
+                  | Success p => f (fst p) (snd p)
+                  | Failure e => Failure e
+                  end.
+  Proof. cbn. unfold Basics.compose. destruct (m s) as [ [a s'] | e]; reflexivity. Qed.
+
+  Lemma stateT_result_ret {A} (a : A) (s : V_map (term V)) :
+    (Mret a : stateT (V_map (term V)) result A) s = Success (a, s).
+  Proof. reflexivity. Qed.
+
+  Section ExtractFixed.
+    Context (g : instance V V V_map V_map V_trie (option positive)).
+    Context (interp : V_map (term V + sort V)).
+    Context (Hsnd : sound interp g).
+
+    Definition cache_sound (cache : V_map (term V)) : Prop :=
+      forall k v, map.get cache k = Some v ->
+        exists ek t, map.get interp k = Some (inl ek) /\ eq_term l [] t v ek.
+
+    Lemma list_extract_sound
+      (rec : V -> stateT (V_map (term V)) Result.result (term V))
+      (Hrec : forall x cache e cache' e_x,
+        cache_sound cache -> map.get interp x = Some (inl e_x) ->
+        rec x cache = Result.Success (e, cache') ->
+        cache_sound cache' /\ exists t, eq_term l [] t e e_x) :
+      forall args args_terms cache children cache',
+        list_Mmap (map.get interp) args = Some (map inl args_terms) ->
+        cache_sound cache ->
+        list_Mmap rec args cache = Result.Success (children, cache') ->
+        cache_sound cache'
+        /\ all2 (fun child e => exists t, eq_term l [] t child e) children args_terms.
+    Proof.
+      induction args as [|a args0 IHargs]; intros args_terms cache children cache' Hget Hcache Hmmap.
+      - cbn in Hmmap. injection Hmmap; intros; subst children cache'.
+        cbn in Hget. destruct args_terms as [|et args_terms0]; [ | cbn in Hget; discriminate ].
+        split; [ exact Hcache | cbn; exact I ].
+      - cbn [list_Mmap] in Hget, Hmmap.
+        destruct (map.get interp a) as [d_a|] eqn:Hia; cbn [Mbind option_monad] in Hget; [ | discriminate ].
+        destruct (list_Mmap (map.get interp) args0) as [ds|] eqn:Hds; cbn [Mbind Mret option_monad] in Hget; [ | discriminate ].
+        injection Hget; intro Heq_dads.
+        destruct args_terms as [|e_a args_terms0]; [ cbn in Heq_dads; discriminate | ].
+        cbn [map] in Heq_dads. injection Heq_dads; intros Hds_eq Hda_eq.
+        rewrite stateT_result_bind in Hmmap.
+        destruct (rec a cache) as [ [c_a cache1] | err1 ] eqn:Hreca; [ cbn [fst snd] in Hmmap | discriminate ].
+        rewrite stateT_result_bind in Hmmap.
+        destruct (list_Mmap rec args0 cache1) as [ [cs cache2] | err2 ] eqn:Hlm; [ cbn [fst snd] in Hmmap | discriminate ].
+        rewrite stateT_result_ret in Hmmap.
+        injection Hmmap; intros Hcache'_eq Hchildren_eq; subst children cache'.
+        assert (Hia' : map.get interp a = Some (inl e_a)) by (rewrite Hia, Hda_eq; reflexivity).
+        destruct (Hrec a cache c_a cache1 e_a Hcache Hia' Hreca) as [Hcache1 Hhead].
+        assert (Hds' : Some ds = Some (map inl args_terms0)) by (rewrite Hds_eq; reflexivity).
+        destruct (IHargs args_terms0 cache1 cs cache2 Hds' Hcache1 Hlm) as [Hcache2 Htail].
+        split; [ exact Hcache2 | ].
+        cbn [all2]. split; [ exact Hhead | exact Htail ].
+    Qed.
+
+    Lemma extractF_sound
+      (rec : V -> stateT (V_map (term V)) Result.result (term V))
+      (Hrec : forall x cache e cache' e_x,
+        cache_sound cache -> map.get interp x = Some (inl e_x) ->
+        rec x cache = Result.Success (e, cache') ->
+        cache_sound cache' /\ exists t, eq_term l [] t e e_x) :
+      forall x cache e cache' e_x,
+        cache_sound cache -> map.get interp x = Some (inl e_x) ->
+        memoizeF (extract_weightedF g) rec x cache = Result.Success (e, cache') ->
+        cache_sound cache' /\ exists t, eq_term l [] t e e_x.
+    Proof.
+      intros x cache e cache' e_x Hcache Hix Hmemo.
+      unfold memoizeF in Hmemo.
+      rewrite stateT_result_bind in Hmemo.
+      unfold stateT_get in Hmemo.
+      cbn [fst snd] in Hmemo.
+      destruct (map.get cache x) as [v|] eqn:Hcx.
+      - cbn [Mret result_monad fst snd] in Hmemo.
+        rewrite Hcx in Hmemo.
+        rewrite stateT_result_ret in Hmemo.
+        injection Hmemo; intros Hc' He; subst e cache'.
+        destruct (Hcache x v Hcx) as (ek & t & Hek & Heqv).
+        rewrite Hix in Hek. injection Hek; intro Hekx; subst ek.
+        split; [ exact Hcache | exists t; exact Heqv ].
+      - cbn [Mret result_monad fst snd] in Hmemo.
+        rewrite Hcx in Hmemo.
+        rewrite stateT_result_bind in Hmemo.
+        unfold extract_weightedF in Hmemo.
+        destruct (map.get (select_optimal_nodes V_map V_trie oP_le (analyses g) (db g)) x) as [ [x_f x_args] | ] eqn:Hopt;
+          cbn [result_of_option_else] in Hmemo; [ | cbn in Hmemo; discriminate ].
+        rewrite stateT_result_bind in Hmemo.
+        cbn [lift stateT_trans Mbind Mret result_monad fst snd] in Hmemo.
+        rewrite stateT_result_bind in Hmemo.
+        destruct (list_Mmap rec x_args cache) as [ [children0 cache_mid] | err ] eqn:Hlm;
+          [ cbn [fst snd] in Hmemo | cbn [fst snd] in Hmemo; discriminate ].
+        rewrite stateT_result_ret in Hmemo.
+        cbn [fst snd] in Hmemo.
+        rewrite stateT_result_bind in Hmemo.
+        unfold stateT_put in Hmemo.
+        cbn [Mret result_monad fst snd] in Hmemo.
+        rewrite stateT_result_ret in Hmemo.
+        injection Hmemo; intros Hcache'_eq He_eq; subst e cache'.
+        pose proof (select_optimal_nodes_sound V V_map V_map_ok V_trie V_trie_ok (option positive) oP_le (analyses g) (db g) x x_f x_args Hopt) as Hatomdb.
+        destruct Hsnd as [Hwf_interp Hexact Hatom_interp Hrel].
+        pose proof (Hatom_interp (Build_atom x_f x_args x) Hatomdb) as Hatomsnd.
+        unfold atom_sound_for_model, Is_Some_satisfying in Hatomsnd.
+        cbn [atom_args atom_ret atom_fn] in Hatomsnd.
+        change (domain V lang_model) with (term V + sort V)%type in Hatomsnd.
+        destruct (list_Mmap (map.get interp) x_args) as [arg_doms|] eqn:Hld;
+          cbn beta iota in Hatomsnd; [ | contradiction ].
+        rewrite Hix in Hatomsnd.
+        change (interprets_to V lang_model) with (lang_model_interprets_to V sort_of l) in Hatomsnd.
+        inversion Hatomsnd as [ | | f0 args0 e0 t0 Heqterm Hf0 Hargs0 He0 ]; subst.
+        destruct (list_extract_sound rec Hrec x_args args0 cache children0 cache_mid Hld Hcache Hlm) as [Hcache_mid Hall].
+        pose proof (eq_term_wf_l wfl ltac:(constructor) Heqterm) as Hwfcon.
+        apply WfCutElim.invert_wf_term_con in Hwfcon.
+        destruct Hwfcon as (c & rule_args & t_rule & Hin & Hwfargs0 & Ht0).
+        assert (Hwfc : wf_ctx (Model:=core_model l) c) by eauto with lang_core.
+        assert (Hall2 : all2 (lang_model_eq V l) (map inl args0) (map inl children0))
+          by (clear -Hall; revert args0 Hall; induction children0 as [|c0 cs' IH];
+              intros [|a0 args0'] Hall; cbn in Hall |- *; try contradiction; auto;
+              destruct Hall as [ [t Ht] Hrest ]; split;
+              [ econstructor; apply eq_term_sym; exact Ht | apply IH; exact Hrest ]).
+        pose proof (all2_model_eq_eq_args V l wfl args0 children0 c Hwfargs0 Hwfc Hall2) as Heqargs.
+        pose proof (term_con_congruence x_f rule_args t_rule Hin (or_intror eq_refl) wfl Heqargs) as Hcong.
+        assert (Hwf1 : wf_term l [] (con x_f args0) (t_rule [/with_names_from c children0 /]))
+          by (apply (eq_term_wf_l wfl ltac:(constructor) Hcong)).
+        assert (Hwf2 : wf_term l [] (con x_f args0) t0)
+          by (apply (eq_term_wf_l wfl ltac:(constructor) Heqterm)).
+        assert (Hsorteq : eq_sort l [] (t_rule [/with_names_from c children0 /]) t0)
+          by (apply (term_sorts_eq wfl ltac:(constructor) Hwf1 Hwf2)).
+        assert (Hfinal : eq_term l [] t0 (con x_f children0) e_x)
+          by (eapply eq_term_trans;
+              [ exact (eq_term_conv (eq_term_sym Hcong) Hsorteq) | exact Heqterm ]).
+        split.
+        + intros k v Hk.
+          destruct (eqb k x) eqn:Hkx; pose proof (eqb_spec k x) as Hkxs; rewrite Hkx in Hkxs.
+          ++ subst k. rewrite map.get_put_same in Hk. injection Hk; intro Hv; subst v.
+             exists e_x, t0. split; [ exact Hix | exact Hfinal ].
+          ++ rewrite map.get_put_diff in Hk; [ | congruence ]. exact (Hcache k v Hk).
+        + exists t0. exact Hfinal.
+    Qed.
+
+    Lemma extract_weighted'_sound :
+      forall efuel x cache e cache' e_x,
+        cache_sound cache -> map.get interp x = Some (inl e_x) ->
+        extract_weighted' g efuel x cache = Result.Success (e, cache') ->
+        cache_sound cache' /\ exists t, eq_term l [] t e e_x.
+    Proof.
+      induction efuel as [|n IHn]; intros x cache e cache' e_x Hcache Hix Hext.
+      - cbn [extract_weighted' decr] in Hext.
+        eapply (extractF_sound default); [ | exact Hcache | exact Hix | exact Hext ].
+        intros x0 cache0 e0 cache0' e_x0 _ _ Hd. cbn in Hd. discriminate Hd.
+      - cbn [extract_weighted' decr] in Hext.
+        eapply (extractF_sound (extract_weighted' g n)); [ exact IHn | exact Hcache | exact Hix | exact Hext ].
+    Qed.
+
+    Lemma extract_weighted_sound (efuel : nat) (x : V) (e : term V) (e_x : term V) :
+      map.get interp (snd (UnionFind.find (equiv g) x)) = Some (inl e_x) ->
+      extract_weighted g efuel x = Result.Success e ->
+      exists t, eq_term l [] t e e_x.
+    Proof.
+      intros Hix Hext.
+      unfold extract_weighted in Hext.
+      cbn [Mbind Mret] in Hext.
+      destruct (extract_weighted' g efuel (snd (UnionFind.find (equiv g) x)) map.empty)
+        as [ [e0 cache0] | err ] eqn:Hext'; cbn [Mbind Mret result_monad fst] in Hext;
+        [ | discriminate ].
+      injection Hext; intro He; subst e0.
+      assert (Hcache0 : cache_sound map.empty)
+        by (intros k v Hk; rewrite map.get_empty in Hk; discriminate).
+      destruct (extract_weighted'_sound efuel _ map.empty e cache0 e_x Hcache0 Hix Hext')
+        as [ _ Heq ].
+      exact Heq.
+    Qed.
+
+  End ExtractFixed.
+
+End Scratch.
+
+Section CongWf.
+  Context (V : Type) {V_Eqb : Eqb V} {V_Eqb_ok : Eqb_ok V_Eqb}.
+  Context (l : Rule.lang V) (wfl : wf_lang l).
+
+  Lemma select_inj_args_wf (c' : ctx V) inj_args (s1 s2 : list (term V)) subgoals :
+    @select_inj_args V V_Eqb c' inj_args s1 s2 = Some subgoals ->
+    wf_args (Model:=core_model l) [] s1 c' ->
+    wf_args (Model:=core_model l) [] s2 c' ->
+    all (fun p => (exists sa, wf_term l [] (fst p) sa)
+                  /\ (exists sb, wf_term l [] (snd p) sb)) subgoals.
+  Proof.
+  Admitted.
+
+  Lemma cong_subgoals_preserves_wf inj_list (e1 e2 : term V) (ta tb : sort V) :
+    wf_term l [] e1 ta -> wf_term l [] e2 tb ->
+    all (fun p => (exists sa, wf_term l [] (fst p) sa)
+                  /\ (exists sb, wf_term l [] (snd p) sb))
+        (@cong_subgoals V V_Eqb l inj_list (e1,e2)).
+  Proof.
+  Admitted.
+
+End CongWf.
+
+Section CongMain.
+  Context (V : Type) {V_Eqb : Eqb V} {V_Eqb_ok : Eqb_ok V_Eqb}
+    {V_default : WithDefault V}.
+  Context (V_map : forall A, map.map V A)
+    (V_map_plus : ExtraMaps.map_plus V_map)
+    (V_map_ok : forall A, map.ok (V_map A))
+    (V_map_plus_ok : ExtraMaps.map_plus_ok V_map)
+    (V_trie : forall A, map.map (list V) A)
+    (V_trie_ok : forall A, map.ok (V_trie A)).
+  Context (succ : V -> V) (sort_of : V) (lt : V -> V -> Prop).
+  Context (lt_asymmetric : Asymmetric lt)
+    (lt_succ : forall x, lt x (succ x))
+    (lt_trans : Transitive lt).
+  Context (spaced_list_intersect
+            : forall B, WithDefault B -> (B -> B -> B) ->
+                        ne_list (V_trie B * list bool) -> V_trie B).
+  Context (l : Rule.lang V) (wfl : wf_lang l) (sort_of_fresh : fresh sort_of l).
+
+  Local Notation lang_model := (lang_model V sort_of l).
+  Local Notation sound :=
+    (egraph_sound_for_interpretation V V V_map V_map V_trie (option positive) lang_model).
+  Local Notation egraph_ok := (egraph_ok V lt V V_map V_map V_trie (option positive)).
+
+  Lemma find_root_denote (g : instance V V V_map V_map V_trie (option positive))
+    (interp : V_map (term V + sort V)) (x : V) (d : term V + sort V) :
+    egraph_ok g -> sound interp g -> map.get interp x = Some d ->
+    exists d', map.get interp (snd (UnionFind.find (equiv g) x)) = Some d'
+               /\ domain_eq V lang_model d' d.
+  Proof.
+    intros Hok Hsnd Hx.
+    assert (Hkey : Sep.has_key x (parent (equiv g)))
+      by (apply (interpretation_exact _ _ _ _ _ _ _ _ _ Hsnd x);
+          change (domain V lang_model) with (term V + sort V)%type; rewrite Hx; exact I).
+    pose proof (find_preserves_fields_strong V V_Eqb V_Eqb_ok lt succ V_default V V_map V_map V_map_ok V_trie (option positive) x g (egraph_equiv_ok _ _ _ _ _ _ _ _ Hok) Hkey) as Hf.
+    destruct (find x g) as [r g'] eqn:Hfind.
+    cbn [fst snd] in Hf.
+    destruct Hf as (Hok' & Hfp & Hrel).
+    destruct Hfp as (_ & _ & _ & _ & _ & Hkiff & Hiff).
+    apply (proj2 (Hiff r x)) in Hrel.
+    pose proof (rel_interpretation _ _ _ _ _ _ _ _ _ Hsnd r x Hrel) as Heqs.
+    unfold eq_sound_for_model, Is_Some_satisfying in Heqs.
+    change (domain V lang_model) with (term V + sort V)%type in Heqs.
+    rewrite Hx in Heqs.
+    destruct (map.get interp r) as [r'|] eqn:Hr; [ | contradiction ].
+    assert (Hreq : snd (UnionFind.find (equiv g) x) = r)
+      by (unfold find in Hfind; destruct (UnionFind.find (equiv g) x) as [uf' v'] eqn:Huf;
+          cbn [snd] in Hfind |- *; congruence).
+    exists r'. rewrite Hreq, Hr. split; [ reflexivity | exact Heqs ].
+  Qed.
+
+  Lemma list_Miter_all_success {A} (f : A -> Result.result unit) (xs : list A) :
+    list_Miter f xs = Result.Success tt -> forall a, In a xs -> f a = Result.Success tt.
+  Proof.
+    induction xs as [|a0 xs' IH]; intros Hm a Hin.
+    - inversion Hin.
+    - cbn [list_Miter] in Hm.
+      destruct (f a0) as [u|err] eqn:Hfa0; cbn [Mbind Mret result_monad] in Hm; [ | discriminate ].
+      destruct Hin as [Heq | Hin'].
+      + subst a. destruct u. exact Hfa0.
+      + exact (IH Hm a Hin').
+  Qed.
+
+  Lemma eq_term_ex_trans (a b c : term V) :
+    (exists s, eq_term l [] s a b) -> (exists s, eq_term l [] s b c) ->
+    exists s, eq_term l [] s a c.
+  Proof.
+    intros [s1 H1] [s2 H2]. exists s1.
+    eapply eq_term_trans; [ exact H1 | ].
+    eapply eq_term_conv; [ exact H2 | ].
+    apply eq_sort_sym.
+    eapply term_sorts_eq;
+      [ exact wfl | constructor
+      | eapply eq_term_wf_r; [ exact wfl | exact H1 ]
+      | eapply eq_term_wf_l; [ exact wfl | exact H2 ] ].
+  Qed.
+
+  Lemma eq_term_ex_sym (a b : term V) :
+    (exists s, eq_term l [] s a b) -> exists s, eq_term l [] s b a.
+  Proof. intros [s H]. exists s. apply eq_term_sym; exact H. Qed.
+
+  Lemma denote_extract_eq (g : instance V V V_map V_map V_trie (option positive))
+    (interp : V_map (term V + sort V)) (efuel : nat) (z : V) (ez efz : term V) :
+    egraph_ok g -> sound interp g ->
+    option_relation (domain_eq V lang_model) (map.get interp z) (Some (inl ez)) ->
+    extract_weighted g efuel z = Result.Success efz ->
+    exists s, eq_term l [] s ez efz.
+  Proof.
+    intros Hokg Hsndg Hrz Hexz.
+    destruct (map.get interp z) as [dz|] eqn:Hiz; [ | unfold option_relation in Hrz; discriminate Hrz ].
+    unfold option_relation in Hrz.
+    destruct (find_root_denote g interp z dz Hokg Hsndg Hiz) as (dz' & Hfz & Hdeq).
+    change (domain_eq V lang_model) with (lang_model_eq V l) in Hrz, Hdeq.
+    inversion Hrz as [ edz ezr srz Htermr Hr1 Hr2 | ]; subst.
+    inversion Hdeq as [ ex edzd sdq Htermd Hd1 Hd2 | ]; subst.
+    destruct (Theorems.extract_weighted_sound V V_map V_map_ok V_trie V_trie_ok sort_of l wfl g interp Hsndg efuel z efz ex Hfz Hexz) as [te Hee].
+    apply (eq_term_ex_trans ez ex efz).
+    - apply (eq_term_ex_trans ez edz ex).
+      + apply eq_term_ex_sym. exists srz. exact Htermr.
+      + apply eq_term_ex_sym. exists sdq. exact Htermd.
+    - apply eq_term_ex_sym. exists te. exact Hee.
+  Qed.
+
+  Lemma egraph_reducing_cong_sound
+    (schedule : list (nat * rule_set V V V_map V_map))
+    (rfuel sat_fuel efuel : nat) :
+    Theorems.schedule_sound_real V V_map V_map_plus V_trie succ sort_of lt spaced_list_intersect l schedule ->
+    forall red_fuel inj goals,
+      (forall a b, In (a,b) goals -> (exists ta, wf_term l [] a ta) /\ (exists tb, wf_term l [] b tb)) ->
+      egraph_reducing_cong V_map_plus V_trie succ sort_of spaced_list_intersect l schedule rfuel sat_fuel efuel red_fuel inj goals = Result.Success tt ->
+      forall a b, In (a,b) goals -> exists s, eq_term l [] s a b.
+  Proof.
+    intros Hsched red_fuel.
+    induction red_fuel as [|rf IHrf]; intros inj goals Hwfgoals Hsucc a b Hin.
+    - cbn [egraph_reducing_cong] in Hsucc. discriminate.
+    - cbn [egraph_reducing_cong] in Hsucc.
+      assert (Hgoals' : forall e1 e2, In (e1,e2) (flat_map (cong_subgoals l inj) goals) -> exists s, eq_term l [] s e1 e2).
+      + intros e1 e2 Hin'.
+        pose proof (list_Miter_all_success _ _ Hsucc (e1,e2) Hin') as Hproc.
+        apply in_flat_map in Hin'. destruct Hin' as [ [a0 b0] [Hin0 Hinsub] ].
+        destruct (Hwfgoals a0 b0 Hin0) as [ [ta0 Hwfa0] [tb0 Hwfb0] ].
+        pose proof (Theorems.cong_subgoals_preserves_wf V l wfl inj a0 b0 ta0 tb0 Hwfa0 Hwfb0) as Hwfsub.
+        pose proof (in_all _ _ _ Hwfsub Hinsub) as Hwfp.
+        cbn [fst snd] in Hwfp. destruct Hwfp as [ [se1 Hwfe1] [se2 Hwfe2] ].
+        cbn beta iota in Hproc.
+        pose proof (Theorems.egraph_reducing_equal_step_sound_strong V V_map V_map_plus V_map_ok V_map_plus_ok V_trie V_trie_ok succ sort_of lt lt_asymmetric lt_succ lt_trans spaced_list_intersect l wfl sort_of_fresh schedule rfuel sat_fuel e1 e2 se1 se2 Hwfe1 Hwfe2 Hsched) as Hstrong.
+        revert Hproc Hstrong.
+        destruct (egraph_reducing_equal_step V_map_plus V_trie succ sort_of spaced_list_intersect l schedule rfuel sat_fuel e1 e2) as [ [ [res x] y] g].
+        intros Hproc [i [Hokg [Hsndg [Hr1 Hr2] ] ] ].
+        destruct res; [ | discriminate Hproc ].
+        assert (Hisx : Is_Some (map.get i x)) by (unfold option_relation in Hr1; destruct (map.get i x); [ exact I | discriminate Hr1 ]).
+        assert (Hisy : Is_Some (map.get i y)) by (unfold option_relation in Hr2; destruct (map.get i y); [ exact I | discriminate Hr2 ]).
+        assert (Hkx : Sep.has_key x (parent (equiv g))) by (exact (interpretation_exact _ _ _ _ _ _ _ _ _ Hsndg x Hisx)).
+        assert (Hky : Sep.has_key y (parent (equiv g))) by (exact (interpretation_exact _ _ _ _ _ _ _ _ _ Hsndg y Hisy)).
+        destruct (are_unified x y g) as [unified pf] eqn:Hau.
+        destruct unified.
+        * pose proof (are_unified_eq_sound V V_Eqb V_Eqb_ok lt succ V_default V V_map V_map V_map_ok V_trie (option positive) lang_model x y g i Hokg Hsndg Hkx Hky ltac:(rewrite Hau; reflexivity)) as Hes.
+          eapply (Theorems.eq_sound_to_eq_term V V_map sort_of l sort_of_fresh wfl i x y e1 e2 Hes); [ exact Hr1 | exact Hr2 ].
+        * destruct (extract_weighted g efuel x) as [e1'|err1] eqn:Hex; cbn [Mbind Mret result_monad] in Hproc; [ | discriminate ].
+          destruct (extract_weighted g efuel y) as [e2'|err2] eqn:Hey; cbn [Mbind Mret result_monad] in Hproc; [ | discriminate ].
+          pose proof (denote_extract_eq g i efuel x e1 e1' Hokg Hsndg Hr1 Hex) as He1.
+          pose proof (denote_extract_eq g i efuel y e2 e2' Hokg Hsndg Hr2 Hey) as He2.
+          assert (Hwfrec : forall aa bb, In (aa,bb) [(e1',e2')] -> (exists ta, wf_term l [] aa ta) /\ (exists tb, wf_term l [] bb tb))
+            by (intros aa bb Hinp; destruct Hinp as [Heqp | Hf]; [ | inversion Hf ];
+                injection Heqp as Haa Hbb; subst; split;
+                [ destruct He1 as [s1 H1]; exists s1; exact (eq_term_wf_r wfl ltac:(constructor) H1)
+                | destruct He2 as [s2 H2]; exists s2; exact (eq_term_wf_r wfl ltac:(constructor) H2) ]).
+          pose proof (IHrf inj [(e1',e2')] Hwfrec Hproc e1' e2' (or_introl eq_refl)) as He12.
+          apply (eq_term_ex_trans e1 e1' e2); [ exact He1 | ].
+          apply (eq_term_ex_trans e1' e2' e2); [ exact He12 | ].
+          apply eq_term_ex_sym. exact He2.
+      + destruct (Hwfgoals a b Hin) as [ [ta Hwfa] [tb Hwfb] ].
+        apply (Theorems.cong_subgoals_sound_ex V l wfl inj a b ta tb Hwfa Hwfb).
+        apply all_via_in_local.
+        intros p Hp. destruct p as [e1 e2].
+        apply (Hgoals' e1 e2).
+        apply in_flat_map. exists (a,b). split; [ exact Hin | exact Hp ].
+  Qed.
+
+  Lemma egraph_reducing_equal_sound_generic
+    (schedule : list (nat * rule_set V V V_map V_map))
+    (rfuel sat_fuel efuel red_fuel : nat) inj (e1 e2 : term V) (t : sort V) :
+    wf_term l [] e1 t -> wf_term l [] e2 t ->
+    Theorems.schedule_sound_real V V_map V_map_plus V_trie succ sort_of lt spaced_list_intersect l schedule ->
+    egraph_reducing_cong V_map_plus V_trie succ sort_of spaced_list_intersect l schedule rfuel sat_fuel efuel red_fuel inj [(e1,e2)] = Result.Success tt ->
+    eq_term l [] t e1 e2.
+  Proof.
+    intros Hwf1 Hwf2 Hsched Hsucc.
+    assert (Hwfg : forall a b, In (a,b) [(e1,e2)] -> (exists ta, wf_term l [] a ta) /\ (exists tb, wf_term l [] b tb))
+      by (intros aa bb Hinp; destruct Hinp as [Heqp | Hf]; [ | inversion Hf ];
+          injection Heqp as Ha Hb; subst; split; [ exists t; exact Hwf1 | exists t; exact Hwf2 ]).
+    destruct (egraph_reducing_cong_sound schedule rfuel sat_fuel efuel Hsched red_fuel inj [(e1,e2)] Hwfg Hsucc e1 e2 (or_introl eq_refl)) as [s Heq].
+    eapply eq_term_conv; [ exact Heq | ].
+    eapply (term_sorts_eq (e := e1)); [ exact wfl | constructor | exact (eq_term_wf_l wfl ltac:(constructor) Heq) | exact Hwf1 ].
+  Qed.
+  (* CONGMAIN-END-MARKER *)
+End CongMain.
